<?xml version="1.0" encoding="UTF-8"?>

<section xml:id="s_caylet_ham" xmlns:xi="http://www.w3.org/2001/XInclude">
    <title>Cayley-Hamilton theorem</title>

    <subsection xml:id="ss_polys">
    <title>Polynomial theory</title>
   <definition xml:id="d_poly_divis">
   <title>Polynomial divisibility</title>
   <statement>
   <p>
   Let <m>F</m> be a field. Recall that <m>P(F)</m> is the set of all polynomials with coefficients in <m>F</m>. 
   <ul>
    <li>
        <title>Divisibility</title>
        <p>
            Given polynomials <m>f,g\in P(F)</m>, we say the <m>g</m> <term>divides</term> <m>f</m> if there is a polynomial <m>q\in P(F)</m> satisfying 
            <men xml:id="eq_poly_div">
                f(x)=q(x)g(x)
            </men>.
            In this case we call <m>f</m> a <term>multiple</term> of <m>g</m>, <m>g</m> a <term>factor</term> of <m>f</m>, and the equation <xref ref="eq_poly_div"/> a <term>factorization</term> of <m>f</m>. 
        </p>
    </li>
    <li>
        <title>Irreducible polynomial</title>
        <p>
            A nonconstant polynomial <m>f\in P(F)</m> is <term>irreducible</term> if it has no nontrivial factorization: more precisely, if <m>f(x)=g_1(x)g_2(x)</m> for <m>g_1,g_2\in F</m>, then <m>g_1(x)</m> is a constant polynomial or <m>g_2(x)</m> is a constant polynomial. 
        </p>
    </li>
    <li>
        <title>Division algorithm</title>
        <p>
            Given polynomials <m>f,g\in P(F)</m> with <m>g\ne \boldzero</m>, there is a unique pair of polynomials <m>(q(x),r(x))</m> satisfying the following conditions: 
            <mdn>
                <mrow xml:id="eq_poly_div_alg">f(x) \amp =q(x)g(x)+r(x)</mrow>
                <mrow xml:id="eq_poly_div_alg_remainder">\deg r(x) \amp &lt; \deg f(x)</mrow>
            </mdn>.
            We call <m>q</m> and <m>r</m> the <term>quotient</term> and <term>remainder</term>, respectively, upon dividing <m>f</m> by <m>g</m>. 
        </p>
    </li>
   </ul>
   </p>
   </statement>
   </definition>
   
    </subsection>
    <subsection xml:id="ss_cayley-ham">
    <title>Cayley-Hamilton theorem</title>
        <theorem xml:id="th_invar_char_poly">
        <title>Invariant subspaces and characteristic polynomial</title>
        <statement>
        <p>
        Let <m>T\in \mathcal{L}(V)</m>, where <m>V</m> is finite dimensional, and suppose <m>W</m> be a <m>T</m>-invariant subspace of <m>V</m>. Let <m>f</m> be the characteristic polynomial of <m>T</m>, and let <m>g</m> be the characteristic polynomial of the restriction <m>T\vert_W</m>. We have <m>g\mid f</m>: <ie/>, the characteristic polynomial of <m>T\vert_W</m> divides the characteristic polynomial of <m>T</m> for any <m>T</m>-invariant subspace <m>W</m>. 
        </p>
        </statement>
        <proof>
        <p>
            Let <m>B'=(v_1,v_2,\dots, v_k)</m> be a basis of <m>W</m>, and extend to a basis <m>B=(v_1,v_2,\dots, v_n)</m>. Since <m>W</m> is <m>T</m>-invariant, it follows easily from <xref ref="eq_matrixrep_formula"/> that
            <me>
                [T]_B=\begin{bmatrix}
                \underset{k\times k}{C} \amp \underset{k\times (n-k)}{D}\\
                \underset{(n-k)\times k}{\boldzero} \amp \underset{(n-k)\times (n-k)}{E}
                \end{bmatrix}
            </me>,
            and that furthermore, <m>C=[T\vert_W]_{B'}</m>.  A matrix of the form <m>A=[T]_B</m> above is called <em>block upper diagonal</em>.  
            An easy induction argument shows that in general the determinant of block upper diagonal matrices is the product of the determinants of the block matrices along the diagonal. As a result we have 
            <md>
                <mrow>\det(xI-A)\amp =\det \begin{bmatrix}
                \underset{k\times k}{xI-C} \amp \underset{k\times (n-k)}{-D}\\
                \underset{(n-k)\times k}{\boldzero} \amp \underset{(n-k)\times (n-k)}{xI-E}
                \end{bmatrix} \amp </mrow>
                <mrow> \amp =\det(xI-C)\det(cI-E)</mrow>
            </md>.
            Since the characteristic polynomial of <m>T</m> is <m>f(x)=\det(xI-A)</m>, and the characteristic polynomial of <m>T\vert_W</m> is <m>g(x)=\det(xI-C)</m> (<m>C=[T\vert_W]_{B'}</m>), we conclude that <m>g\mid f</m>.
        </p>
        </proof>
        </theorem>
        



    
    
    <definition xml:id="d_multiplicity">
    <title>Multiplicity</title>
    <statement>
    <p>
    Let <m>f\in P(F)</m>. 

                Suppose <m>c\in F</m> is a root of <m>f</m> and let 
                <me>
                    f(x)=(x-c)^mg(x)
                </me>
                be a factorization of <m>f</m> satisfying <m>g(c)\ne 0</m>. The integer <m>m</m> is called the <term>multiplicity</term> of the root <m>c</m>.
    </p>
    </statement>
    </definition>
    <definition xml:id="d_multiplicity_eigenvalues">
    <title>Multiplicity of eigenvalues</title>
    <statement>
    <p>
    Let <m>T\in \mathcal{L}(V)</m>, where <m>V</m> is finite dimensional, let <m>f\in P(F)</m> be the characteristic polynomial of <m>T</m>, and let <m>\lambda</m> be an eigenvalue of <m>T</m>. 
    <ul>
        <li>
            <title>Algebraic multiplicity</title>
            <p>
                The <term>algebraic multiplicity</term> of <m>\lambda</m> is its multiplicity as a root of <m>f</m>: <ie/> the algebraic multiplicity of <m>\lambda</m> is the positive integer <m>m</m> such that <m>f(x)=(x-\lambda)^mg(x)</m> for some <m>g\in P(F)</m> satisfying <m>g(\lambda)\ne 0</m>. 
            </p>
        </li>
        <li>
            <title>Geometric multiplicity</title>
            <p>
                The <term>geometric multiplicity</term> of <m>\lambda</m> is defined as <m>\dim E(\lambda, T)</m>. 
            </p>
        </li>
    </ul>
    </p>
    </statement>
    </definition>
    <corollary xml:id="cor_alg_geom_mult">
        <statement>
            <p>
                Let <m>T\in \mathcal{L}(V)</m>, where <m>V</m> is finite dimensional, let <m>f\in P(F)</m> be the characteristic polynomial of <m>T</m>. Let <m>\lambda</m> be an eigenvalue of <m>T</m> of algebraic multiplicity <m>m</m>: <ie/>, suppose <m>f</m> factors as 
                <me>
                    f(x)=(x-\lambda)^mg(x)
                </me>,
                where <m>g(\lambda)\ne 0</m>. 
                The geometric multiplicity of <m>\lambda</m> is bounded above by the algebraic multiplicity: <ie/>, 
                    <men xml:id="eq_alg_geom_mult">
                        \dim E(\lambda, T)\leq m
                    </men>. 
            </p>
        </statement>
    </corollary>
    <proof>
        <p>
            Let <m>W=E(\lambda, T)</m>. Since <m>[T\vert_W]_B</m> is diagonal (with diagonal entries <m>\lambda</m>), for any basis <m>B</m> of <m>W</m>, we see that the characteristic polynomial of <m>T\vert_W</m> is 
            <me>
                h(x)=(x-\lambda)^{\dim W}=(x-\lambda)^{\dim E(\lambda, T)}
            </me>.
            (Recall that the degree of a characteristic polynomial is always equal to the dimension of the underlying space.) By <xref ref="th_invar_char_poly"/>, we have <m>h\mid f</m>. Since <m>g(\lambda)\ne 0</m>, we cannot have <m>h\mid g</m>, and thus <m>h\mid  (x-\lambda)^m</m>. (This is intuitive enough, but is actually a consequence of the uniqueness claim of <xref ref="th_factorization_polynomials"/>.) But if 
            <me>
                (x-\lambda)^{\dim E(\lambda, T)}\mid (x-\lambda)^m
            </me>,
            it follows (again by unique factorization) that <m>\dim E(\lambda, T)\leq m</m>. 
        </p>
    </proof>
    

    <definition xml:id="d_Tcyclic_subspace">
    <title><m>T</m>-cyclic subspace</title>
    <statement>
    <p>
    Let <m>T\in \mathcal{L}(V)</m>. Given a vector <m>v\in V</m>, the <term><m>T</m>-cyclic subspace generated by <m>v</m></term> is defined as 
    <me>
        \Span(T^i(v))_{i=0}^\infty=\Span(v,T(v),T^2(v),\dots )
    </me>.
    </p>
    </statement>
    </definition>
    <theorem xml:id="th_Tcyclic_sub">
    <title><m>T</m>-cyclic subspace</title>
    <statement>
    <p>
    Let <m>T\in \mathcal{L}(V)</m>, let <m>v\in V</m> be nonzero, and let <m>W=\Span(T^i(v))_{i=0}^\infty</m>.
    <ol>
        <li>
            <p>
                <m>W</m> is a <m>T</m>-invariant subspace of <m>V</m>. 
            </p>
        </li>
        <li>
            <p>
                If <m>W'</m> is a <m>T</m>-invariant subspace of <m>V</m> containing <m>v</m>,  then <m>W\subseteq W'</m>: <ie/>, <m>W</m> is the smallest <m>T</m>-invariant subspace of <m>V</m> containing <m>v</m>. 
            </p>
        </li>
        <li>
            <p>
                If <m>\dim W&lt; \infty</m>, then there is a <m>k\geq 0</m> such that 
                <me>
                    B=(T^{i}(v))_{i=0}^{k-1}=(v,T(v),\dots, T^{k-1}(v))
                </me>
                is a basis of <m>W</m>.
            </p>
        </li>
    </ol>
    </p>
    </statement>
    <proof>
    <p>
        <ol>
            <li>
                <p>
                    This is left to the reader. 
                </p>
            </li>
            <li>
                <p>
                    Assume <m>W'</m> is a <m>T</m>-invariant subspace containing <m>v</m>. Since <m>W'</m> is <m>T</m>-invariant, it contains <m>T^{i}(v)</m> for all <m>i\in \Z_{\geq 0}</m>. By <xref ref="th_span"/>, we have 
                    <me>
                        W=\Span(T^i(v))_{i=0}^\infty\subseteq W'
                    </me>.
                </p>
            </li>
            <li>
                <p>
                If <m>W</m> is finite dimensional, then the tuple <m>(T^i(v))_{i=0}^\infty</m> must be linearly dependent. It follows that  <m>T^k(v)</m> can be written as a linear combination of the previous <m>T^i(v)</m> for some <m>k\in \Z_{\geq 1}</m> (<m>v</m> is assumed to be nonzero). Let <m>k</m> be minimal in this respect. The tuple <m>B=(v,T(v),\dots, T^{k-1}(v))</m> is then linearly independent by <xref ref="cor_span_ind"/>.  We claim <m>B</m> spans <m>W</m>, and hence is a basis. Since <m>\Span B\subseteq W</m> by definition, we need only show that <m>W\subseteq \Span B</m>. By the previous result it suffices to show that <m>W</m> is <m>T</m>-invariant (since <m>v\in W</m>). This is easy: given any <m>v\in \Span B</m>, we have <m>v=\sum_{i=0}^{k-1}a_iT^i(v)</m> for some <m>a_i</m>, in which case 
                <me>
                    T(v)=\sum_{i=0}^{k-1}a_iT^{i+1}(v_i)=\sum_{i=1}^{k-1}a_{i-1}T^i(v)+T^k(v)\in \Span B
                </me>,
                since <m>\sum_{i=1}^{k-1}a_{i-1}T^i(v)\in \Span B</m> and <m>T^k(v)\in \Span B</m>.
                </p>
            </li>
        </ol>
    </p>
    </proof>
    </theorem>

    <theorem xml:id="th_cayley_ham">
    <title>Cayley-Hamilton theorem</title>
    <statement>
    <p>
    Let <m>T\in\mathcal{L}(V)</m>, where <m>V</m> is finite dimensional, and let <m>f\in P(F)</m> be the characteristic polynomial of <m>T</m>. We have 
    <men xml:id="eq_cayley_ham">
        f(T)=0_V
    </men>.
    In other words, <m>T</m> is a <q>root</q> of its own characteristic polynomial. 
    </p>
    </statement>
    <proof>
    <p>
        It suffices to show that <m>f(T)(v)=\boldzero</m> for all <m>v\in V</m>. This is clearly true for <m>v=\boldzero</m>. Let <m>v\in V</m> be nonzero and let <m>W=\Span (T^i(v))_{i=0}^\infty</m> be the <m>T</m>-cyclic subspace it generates. By <xref ref="th_Tcyclic_sub"/>, <m>W</m> has a basis <m>B</m> of the form 
        <me>
            B=(v,T(v), \dots, T^{k-1}(v))
        </me>
        for some <m>k</m>, in which case <m>\dim W=\len B=k</m>, and we have 
        <me>
            T^k(v)=a_0v+a_1T(v)+\cdots +T^{k-1}(v)
        </me>
        for some scalars <m>a_i\in F</m>. From the nature of <m>B</m>, and the representation of <m>T^k(v)</m> above, it follows that the restriction <m>T\vert_W</m> has matrix representation
        <me>
            A=[T\vert_W]_B=\begin{bmatrix}
            0\amp 0\amp \dots \amp 0 \amp a_0\\
            1\amp 0 \amp \amp \amp a_1 \\ 
            0\amp 1 \amp \ddots\amp \amp \vdots\\ 
            \vdots \amp \amp \ddots \amp 0 \amp  \\ 
            0 \amp \dots\amp 0 \amp 1 \amp a_{k-1} 
            \end{bmatrix}
        </me>.
        An easy proof by induction shows that the characteristic polynomial of a matrix like <m>A</m> is 
        <me>
            g(x)=x^k-a_{k-1}x^{k-1}+\cdots +a_1x+a_0
        </me>.
        Note that 
        <me>
            g(T)(v)=T^k(v)-a_{k-1}T^{k-1}+\cdots +a_1T+a_0v=\boldzero
        </me>
        since <m>T^k(v)=\sum_{i=0}^{k-1}a_iT^i(v)</m>. Lastly, since <m>g\mid f</m> by <xref ref="th_invar_char_poly"/>, we have <m>f(x)=q(x)g(x)</m> for some polynomial <m>q\in P(F)</m>, and hence
        <me>
            f(T)(v)=q(T)g(T)(v)=q(T)(\boldzero)=\boldzero
        </me>,
        as desired.
    </p>
    </proof>
    </theorem>
    
    
    </subsection>
    <subsection xml:id="ss_min_poly">
    <title>Minimal polynomial</title>
    <definition xml:id="d_min_poly">
    <title>Minimal polynomial</title>
    <statement>
    <p>
    Let <m>T\in\mathcal{L}(V)</m>, where <m>V</m> is finite dimensional. The <term>minimal polynomial</term> of <m>T</m> is the unique monic polynomial <m>m_T(x)</m> of minimal degree satisfying <m>m_T(T)=0_V</m>. 
    </p>
    </statement>
    </definition>
    <theorem xml:id="th_min_poly">
    <title>Minimal polynomial</title>
    <statement>
    <p>
    Let <m>T\in \mathcal{L}(V)</m>, where <m>V</m> is finite dimensional and let <m>m_T(x)</m> be the minimal polymonial of <m>T</m>. If <m>g\in P(F)</m> satisfies <m>g(T)=0_V</m>, then <m>m_T\mid g</m>: <ie/>, we have 
        <me>
            g(x)=q(x)m_T(x)
        </me>
        for some <m>q\in P(F)</m>. In particular, if <m>f</m> is the characteristic polynomial of <m>g</m>, then <m>m_T(x)\mid f</m>. 
    </p>
    </statement>
    <proof>
    <p>
        Assume <m>g(T)=0_V</m> for the polynomial <m>g\in P(F)</m>. Using the division algorithm (<xref ref="d_poly_divis"/>), we can write 
        <me>
            g(x)=q(x)m_T(x)+r(x)
        </me>,
        where <m>\deg r(x)^lt; \deg m_T(x)</m>. We thus have 
        <me>
            0_V=g(T)=q(T)m_T(T)+r(T)=q(T)0_V+r(T)=r(T)
        </me>.
        Thus <m>r(T)=0_V</m>. Since by definition <m>m_T(x)</m> is the nonconstant polynomial of minimal degree satisfying <m>m_T(T)=0_V</m>, we conclude that <m>r(x)</m> is a constant polynomial. Since <m>r(T)=0_V</m>, it follows that <m>r(x)=0</m>, the zero polynomial. But then <m>g(x)=q(x)m_T(x)</m>, showing that <m>m_T\mid g</m>, as desired.
    </p>
    </proof>
    </theorem>
    <corollary xml:id="cor_min_poly">
        <title>Minimal polynomial and characteristic polynomial</title>
        <statement>
            <p>
                Let <m>T\in \mathcal{L}(V)</m>, where <m>V</m> is finite dimensional, let <m>f</m> and <m>m_T</m> be the characteristic and minimal polynomials of <m>T</m>, respectively. If <m>f</m> splits completely over <m>F</m> as 
                <me>
                    f(x)=\prod_{i=1}^r(x-\lambda_i)^{n_i}, n_i\geq 1
                </me>,
                then <m>m_T(x)</m> splits completely as 
                <me>
                    m_T(x)=\prod_{i=1}^{r}(x-\lambda_i)^{m_i}
                </me>,
                where <m>1\leq m_i\leq n_i</m> for all <m>1\leq i\leq r</m>. In other words, <m>m_T</m> and <m>f</m> both split completely over <m>F</m> and have the same set of roots.
            </p>
        </statement>
        <proof>
            <p>
                Since <m>m_T\mid f</m>, unique factorization of polynomials implies 
                <me>
                    m_T(x)=\prod_{j\in J}(x-\lambda_{j})^{m_{j}}
                </me>
                for some subset <m>J\subseteq I=\{1,2,\dots, r\}</m>, and exponents <m>m_{j}\leq n_{j}</m>. We will show that <m>J=I</m>: equivalently, we will show that <m>(x-\lambda_i)\mid m_T(x)</m> for all <m>1\leq i\leq r</m>. Fix <m>1\leq i\leq r</m> and eigenvector <m>v\in E(\lambda_i, T)</m>. Since <m>T(v)=\lambda_i v</m>, we have <m>(T-\lambda I)v=(\lambda_i-\lambda)v</m>, and hence <m>(T-\lambda I)^k(v)=(\lambda_i-\lambda)^kv</m>. It follows that 
                <md>
                    <mrow>m_T(T)(v) \amp =\prod_{j\in J}(T-\lambda_j)^{m_{j}}(v)</mrow>
                    <mrow> \amp = \left(\prod_{j\in J}(\lambda_i-\lambda_{j})^{m_{j}}\right)v</mrow>
                </md>
                Since <m>m_T(T)(v)=\boldzero</m>, and since <m>v\ne \boldzero</m>, we must have 
                <me>
                    \prod_{j\in J}(\lambda_i-\lambda_{j})^{m_{j}}=0
                </me>.
                But this is true if and only if <m>\lambda_i=\lambda_{j}</m> for some <m>j\in J</m>, or equivalently, <m>i\in J</m>.
            </p>
        </proof>
    </corollary>
    
    
    
    </subsection>
</section>