<?xml version="1.0" encoding="UTF-8"?>

<section xml:id="s_normal" xmlns:xi="http://www.w3.org/2001/XInclude">
    <title>Normal operators</title>

    <definition xml:id="d_normal">
    <title>Normal operator</title>
    <statement>
    <p>
    Let <m>T</m> be a linear operator on the inner product space <m>(V,\angvec{\, ,})</m>, and suppose <m>T</m> has an adjoint <m>T^*</m>. We say <m>T</m> is <term>normal</term> if it commutes with <m>T^*</m>: <ie/>, if <m>T*T=TT^*</m>. 
    </p>
    </statement>
    </definition>
    <definition xml:id="d_normal_egs">
    <title>Self-adjoint, skew-Hermitian, unitary</title>
    <statement>
    <p>
    Let <m>(V,\angvec{\, ,})</m> be an inner product space. Below we define several special types of normal operators. Let <m>T\in \mathcal{L}(V)</m> and suppose <m>T</m> has an adjoint <m>T^*</m>. 
    <ul>
        <li>
            <title>Self-adjoint</title>
            <p>
                <m>T</m> is <term>self-adjoint</term> (or <term>symmetric</term> when <m>F=\R</m>) if <m>T^*=T</m>. 
            </p>
        </li>
        <li>
            <title>Skew-Hermitian</title>
            <p>
                <m>T\in \mathcal{L}(V)</m> is <term>skew-Hermitian</term> (or <term>skew-symmetric</term> when <m>F=\R</m>) if <m>T^*=-T</m>.
            </p>
        </li>
        <li>
            <title>Unitary</title>
            <p>
                <m>T\in \mathcal{L}(V)</m> is <term>unitary</term> (or <term>orthogonal</term> when <m>F=\R</m>) if <m>T</m> is invertible and <m>T^{-1}=T^*</m>. 
            </p>
        </li>
    </ul>
    </p>
    </statement>
    </definition>
    <remark>
        <title>Self-adjoint, skew-Hermitian, unitary</title>
        <p>
            To show each of the subtypes described in <xref ref="d_normal_egs"/> is indeed normal we simply have to show that an operator of a given type satisfies <m>T^*T=TT^*</m>. This is not difficult: 
            <md>
                <mrow> \text{Self-adjoint}: T^*=T \amp \implies T^*T=TT=TT^*</mrow>
                <mrow>\text{Skew-Hermitian}: T^*=-T \amp \implies T^*T=-TT=T(-T)=TT^*</mrow>
                <mrow>\text{Unitary}: T^*=T^{-1} \amp \implies T^*T=T^{-1}T=I=TT^{-1}=TT^*</mrow>
            </md>.
        </p>
        
    </remark>

    <example xml:id="eg_ortho_proj">
    <title>Orthogonal projection</title>
    <statement>
    <p>
    Let <m>W</m> be a finite-dimensional subspace of the inner product space <m>(V,\angvec{\, ,})</m>, and let <m>\proj_W\colon V\rightarrow V</m> be orthogonal projection onto <m>W</m>. Show that <m>\proj_W</m> is self-adjoint. 
    </p>
    </statement>
    <solution>
    <p>
        This is part of a homework exercise. 
    </p>
        <!-- <p>
    Since <m>\dim W&lt; \infty</m>, we have <m>V=W\oplus W^\perp</m> and can decompose every vector <m>v\in V</m> in a unique way as <m>v=\proj_W(v)+\proj_{W^\perp}(v)</m>, where <m>\proj_W(v)\in V</m> and <m>\proj_{W^\perp}(v)\in W^\perp</m>. It follows that for any <m>v,v'\in V</m>, we have 
    <md>
        <mrow> \angvec{\proj_W(v),v'} \amp = \angvec{\proj_W(v),\proj_W(v')+\proj_{W^\perp}(v')}</mrow>
        <mrow> \amp = \angvec{\proj_W(V),\proj_W(v')} \amp (\proj_{W^\perp}(v')\in W^\perp)</mrow>
        <mrow> \amp = \angvec{\proj_W(v)+\proj_{W^\perp}(v),\proj_{W}(v')} \amp (\proj_{W^\perp}(v)\in W^\perp)</mrow>
        <mrow> \amp =\angvec{v,\proj_W(v')}</mrow>
    </md>.
    This shows that <m>\proj_W</m> satisfies the adjoint property with respect to itself, and hence that <m>(\proj_W)^*=\proj_W</m>. 
    
    </p> -->
    </solution>
    </example>
    <example xml:id="eg_derivative_skew-symm">
    <title>Derivative operator</title>
    <statement>
    <p>
    Let <m>W</m> be the subspace of real periodic <m>C^\infty</m> functions on <m>\R</m> with period <m>1</m>. Recall that the derivative operator <m>T\in \mathcal{L}(W)</m> defined as <m>T(f)=f'</m> has adjoint <m>T^*-T</m> with respect to the inner product <m>\angvec{f,g}=\int_0^1f(x)g(x)\, dx</m>. Hence <m>T</m> is skew-symmetric. In particular, <m>T</m> is normal. 
    </p>
    </statement>
     </example>
    <p>
        The following matrix-based result gives us an easy way of producing normal operators of varying types. 
    </p>
    <theorem xml:id="th_normal_matrix_rep">
    <title>Normality and matrix representations</title>
    <statement>
    <p>
    Let <m>(V,\angvec{\, ,})</m> be a finite-dimensional inner product space, let <m>T\in \mathcal{L}(V)</m>, let <m>B</m> be an <em>orthonormal</em> basis of <m>V</m>, and let <m>A=[T]_B</m>.  
    <ul>
        <li>
            <p>
                <m>T</m> is normal if and only if <m>A^*A=AA^*</m>.
            </p>
        </li>
        <li>
            <p>
                <m>T</m> is self-adjoint if and only if <m>A^*=A</m>.
            </p>
        </li>
        <li>
            <p>
                <m>T</m> is skew-symmetric if and only if <m>A^*=-A</m>.
            </p>
        </li>
        <li>
            <p>
                <m>T</m> is unitary if and only if <m>A</m> is invertible and  <m>A^*=A^{-1}</m>.
            </p>
        </li>
    </ul> 
    </p>
    </statement>
    <proof>
    <p>
        The equivalences are simple consequences of the following facts: 
        <ul>
            <li>
                <p>
                    <m>[TS]_B=[T]_B[S]_B</m> for all <m>S,T\in \mathcal{L}(V)</m> (<xref ref="cor_matrix_reps_comp"/>);
                </p>
            </li>
            <li>
                <p>
                    <m>[T^*]_B=[T]_B^*</m> for all <m>T\in \mathcal{L}(V)</m> (<xref ref="cor_adj_matrix_reps"/>).
                </p>
            </li>
        </ul>
    </p>
    </proof>
    </theorem>
    <p>
        The next theorem tells us that these various types of normality are preserved by familiar operations on linear transformations. 
    </p>
    <theorem xml:id="th_normal_preserved">
    <title>Normality preserved</title>
    <statement>
    <p>
    Let <m>(V,\angvec{\, ,})</m> be an inner product space. Let <m>\operatorname{Norm}(V)</m>, <m>\operatorname{Sym}(V)</m>, <m>\operatorname{Skew}(V)</m>, and <m>\operatorname{Uni}(V)</m> denote the sets of normal, self-adjoint, skew-Hermitian, and unitary operators on <m>V</m>, respectively, and let <m>\mathcal{P}</m> denote any one of these sets of operators. 
    <ol>
        <li>
            <p>
                <m>T\in \mathcal{P}</m> if and only if <m>T^*\in \mathcal{P}</m>. 
            </p>
        </li>
        <li>
            <p>
                If <m>S,T\in\mathcal{P}</m>, then <m>cS+dT\in \mathcal{P}</m> for all <m>c,d\in F</m>. 
            </p>
        </li>
        <li>
            <p>
                If <m>T\in \mathcal{P}</m>, then <m>T^k\in \mathcal{P}</m> for any positive integer <m>k</m>.
            </p>
        </li>
        
    </ol>
    </p>
    </statement>
    <proof>
    <p>
        The statements follow easily from elementary properties of the adjoint (<xref ref="th_adjoint_props"/>).
    </p>
    </proof>
    </theorem>
    <theorem xml:id="th_polar_identities">
    <title>Polar identities</title>
    <statement>
    <p>
    Let <m>(V,\angvec{\, ,})</m> be an inner product space. For all <m>v,w\in V</m>, we have 
    <men xml:id="eq_polar_id">
        \angvec{v,w}=\frac{1}{4}(\norm{v+w}^2-\norm{v-w}^2)+\frac{1}{4}(\norm{v+iw}^2-\norm{v-iw}^2)\, i
    </men>,
    or equivalently, 
    <mdn>
        <mrow xml:id="eq_polar_id_real_part">\Re \angvec{v,w} \amp = \frac{1}{4}(\norm{v+w}^2-\norm{v-w}^2)</mrow>
        <mrow xml:id="eq_polar_id_im_part">\Im \angvec{v,w} \amp = \frac{1}{4}(\norm{v+iw}^2-\norm{v-iw}^2) </mrow>
    </mdn>.
    As a consequence, if <m>F=\R</m>, then we have 
    <men xml:id="eq_polar_id_reals">
        \angvec{v,w}=\frac{1}{4}(\norm{v+w}^2-\norm{v-w}^2)
    </men>.
    </p>
    </statement>
    <proof>
    <p>
       This is a simple, if somewhat tedious exercise of expanding out the right side of <xref ref="eq_polar_id"/> using the definition <m>\norm{u}^2=\angvec{u,u}</m>, and then simplifying using properties of the inner product, and the fact that 
       <md>
        <mrow>\Re z \amp =\frac{1}{2}(z+\overline{z})</mrow>
        <mrow>\Im z \amp =\frac{1}{2i}(z-\overline{z})</mrow>
       </md>
       for all <m>z\in \C</m>. 
    </p>
    </proof>
    </theorem>
    <theorem xml:id="th_normal_equiv">
    <title>Normality equivalence</title>
    <statement>
    <p>
    Let <m>T</m> be a linear operator on the inner product space <m>(V,\angvec{\, ,})</m>. The following statements are equivalent. 
    <ol>
        <li>
            <p>
                <m>T</m> is normal.
            </p>
        </li>
        <li>
            <p>
                <m>\norm{T(v)}=\norm{T^*(v)}</m> for all <m>v\in V</m>.
            </p>
        </li>
        <li>
            <p>
                <m>\angvec{T(v),T(w)}=\angvec{T^*(v),T^*(w)}</m> for all <m>v\in V</m>. 
            </p>
        </li>
    </ol>
    </p>
    </statement>
    <proof>
    <p>
        We prove a cycle of implications. 
    </p>
    <p>
        If <m>T</m> is normal, then 
        <md>
            <mrow>\norm{T(v)}^2 \amp =\angvec{T(v),T(v)}</mrow>
            <mrow> \amp =\angvec{v,T^*Tv}</mrow>
            <mrow> \amp =\angvec{v,TT^*v} \amp (T^*T=TT^*)</mrow>
            <mrow> \amp =\angvec{T^*(v),T^*(v)}</mrow>
            <mrow> \amp =\norm{T^*(v)}^2</mrow>
        </md>.
        Taking square-roots of both sides (and using the fact that norms are nonnegative), we conclude that <m>\norm{T(v)}=\norm{T^*(v)}</m>. This proves (1)<m>\implies</m>(2). 
    </p>
    <p>
        To prove (2)<m>\implies</m>(3), we use the polarity identity. If <m>\norm{T(v)}=\norm{T^*(v)}</m> for all <m>v\in V</m>, then we have 
        <md>
            <mrow>\angvec{T(v),T(w)} \amp = \frac{1}{4}(\norm{T(v)+T(w)}^2-\norm{T(v)-T(w)}^2)+\frac{1}{4}(\norm{T(v)+iT(w)}^2-\norm{T(v)-iT(w)}^2)i</mrow>
            <mrow> \amp =\frac{1}{4}(\norm{(T(v+w))}^2-\norm{T(v-w)}^2)+\frac{1}{4}(\norm{T(v+iw)}^2-\norm{T(v-iw)}^2)i</mrow>
            <mrow> \amp = \frac{1}{4}(\norm{(T^*(v+w))}^2-\norm{T^*(v-w)}^2)+\frac{1}{4}(\norm{T^*(v+iw)}^2-\norm{T^*(v-iw)}^2)i</mrow>
            <mrow> \amp =\frac{1}{4}(\norm{T^*(v)+T^*(w)}^2-\norm{T^*(v)-T^*(w)}^2)+\frac{1}{4}(\norm{T^*(v)+\overline{i}T^*(w)}^2-\norm{T^*(v)-\overline{i}T^*(w)}^2)i </mrow>
            <mrow> \amp = \angvec{T^*(v),T^*(w)}</mrow>
        </md>
    </p>
    </proof>
    </theorem>
    <corollary xml:id="cor_normal_props">
        <title>Normal operator properties</title>
        <statement>
            <p>
               Let <m>(V,\angvec{\, ,})</m> be an inner product space, and assume <m>T\in \mathcal{L}(V)</m> is normal. 
                <ol>
                    <li>
                        <p>
                           <m>T(v)=\boldzero</m> if and only if <m>T^*(v)=\boldzero</m>. As a consequence, we have <men xml:id="eq_normal_null">\NS T=\NS T^*</men>.
                        </p>
                    </li>
                    <li>
                        <p>
                            <m>T(v)=\lambda v</m> if and only if <m>T^*(v)=\overline{\lambda}v</m>. As a consequence, we have 
                            <men xml:id="eq_normal_eigenspace">
                                E(\lambda, T)=E(\overline{\lambda},T^*)
                            </men>
                            for all <m>\lambda\in F</m>.
                        </p>
                    </li>
                    <li>
                        <title>Finite-dimensional space</title>
                        <p>
                            Assume further that <m>\dim V=n&lt; \infty</m>. We have 
                            <men xml:id="eq_normal_image">
                                \im T=\im T^*
                            </men>
                            and 
                            <men xml:id="eq_normal_direct_sum">
                                V=\ker T\oplus \im T=\ker T^*\oplus \im T^*
                            </men>.
                        </p>
                    </li>
                </ol>
            </p>
        </statement>
        <proof>
            <p>
                Assume <m>T</m> is normal. 
            <ol>
                <li>
                    <p>
                        We have 
                        <md>
                            <mrow>v\in \NS T \amp \iff T(v)=\boldzero</mrow>
                            <mrow> \amp \iff \norm{T(v)}=0</mrow>
                            <mrow> \amp \iff \norm{T^*(v)}=0</mrow>
                            <mrow> \amp \iff T^*(v)=\boldzero</mrow>
                            <mrow> \amp \iff v\in \NS T^*</mrow>
                        </md>.
                        Thus <m>\NS T=\NS T^*</m>. 
                    </p>
                </li>
                <li>
                    <p>
                        Since <m>T</m> and <m>I_V</m> are normal, so is, <m>\lambda I_V-T</m> for any <m>\lambda\in F</m> by <xref ref="th_normal_preserved"/>. Applying the result in (1) to <m>\lambda I_V-T</m>, we have 
                        <md>
                            <mrow>T(v)=\lambda v \amp \iff v\in E(\lambda, T) </mrow>
                            <mrow> \amp \iff v\in \NS (\lambda I_V-T)</mrow>
                            <mrow> \amp \iff v\in \NS(\lambda I_V-T)^*</mrow>
                            <mrow> \amp \iff v\in \NS(\overline{\lambda}I_V-T^*) \amp <xref ref="th_adjoint_props"/> </mrow>
                            <mrow> \amp \iff v\in E(\overline{\lambda},T^*) </mrow>
                            <mrow> \amp \iff T^*(v)=\overline{\lambda}v</mrow>
                        </md>.
                    </p>
                </li>
                <li>
                    <p>
                        If we assume <m>V</m> is finite dimensional, then we have 
                        <md>
                            <mrow>\im T^* \amp =(\NS T)^\perp</mrow>
                            <mrow> \amp =(\NS T^*)^\perp</mrow>
                            <mrow> \amp = ((\im T)^\perp)^\perp</mrow>
                            <mrow> \amp =\im T</mrow>
                        </md>.
                        It follows that 
                        <md>
                            <mrow>V \amp = \NS T\oplus (\NS T)^\perp</mrow>
                            <mrow> \amp = \NS T \oplus \im T^*</mrow>
                            <mrow> \amp =\NS T\oplus \im T</mrow>
                            <mrow> \amp =\NS T^*\oplus \im T^*</mrow>
                        </md>.
                    </p>
                </li>
            </ol>
            </p>
        </proof>
    </corollary>
    
    
   
    
    
    

</section>