<?xml version="1.0" encoding="UTF-8"?>

<section xml:id="s_subspace_sum" xmlns:xi="http://www.w3.org/2001/XInclude">
    <title>Subspace sums</title>

    <definition xml:id="d_vec_ops_sets">
    <title>Vector operations on sets</title>
    <statement>
    <p>
    Let <m>V</m> be an <m>F</m>-vector space. Given subsets <m>X_1,X_2,\dots, X_n</m> of <m>V</m>, we define their <term>sum</term>, denoted <m>X_1+X_2+\cdots +X_n</m> or <m>\sum_{i=1}^nX_i</m>, as 
    <me>
        X_1+X_2+\cdots +X_n=\{v_1+v_2+\cdots +v_n\colon v_i\in X_i\}
    </me>.
    Similarly, given a set <m>X\subseteq V</m> and scalar <m>c\in F</m>, we define the <term>scalar multiple</term> <m>cX</m> as 
    <me>
        cX=\{cv\colon v\in X\}
    </me>.
    </p>
    </statement>
    </definition>
    <theorem xml:id="th_subspace_sum">
    <title>Sum of subspaces</title>
    <statement>
    <p>
    Let <m>W_1, W_2, \dots, W_n</m> be subspaces of the <m>F</m>-vector space <m>V</m>, and let <m>W=\sum_{i=1}^n W_i</m> be their sum.
    <ol>
        <li>
            <p>
                <m>W</m> is a subspace of <m>V</m>. 
            </p>
        </li>
        <li>
            <p>
                <m>W</m> is the <em>smallest subspace</em> of <m>V</m> satisfying <m>W_i\subseteq W </m> for all <m>1\leq i\leq n</m> in the following sense: if <m>U</m> is a subspace of <m>V</m> satisfying <m>W_i\subseteq U</m> for all <m>1\leq i\leq n</m>, then <m>W\subseteq U</m>. 
            </p>
        </li>
    </ol>
    </p>
    </statement>
    <proof>
    <p>
    <ol>
        <li>
            <p>
                We follow <xref ref="proc_subspace"/>. 
            </p>
            <p>
                Since <m>\boldzero\in W_i</m> for all <m>1\leq i\leq n</m>, and since 
                <me>
                    \boldzero=\underset{W_1}{\boldzero}+\underset{W_2}{\boldzero}+\cdots +\underset{W_n}{\boldzero}
                </me>,
                we see that <m>\boldzero\in W=\sum_{i=1}^n W_i</m>.
            </p>
            <p>
                Assume <m>w_1, w_2\in W</m>. By definition, we have 
                <md>
                    <mrow>w_1 \amp =v_1+v_2+\cdots +v_n, v_i\in W_i</mrow>
                    <mrow>w_2 \amp =v_1'+v_2'+\cdots +v_n', v_i'\in W_i</mrow>
                </md>.
                But then for any scalars <m>c,d\in F</m>, we have 
                <md>
                    <mrow>cw_1+dw_2 \amp = c(v_1+v_2+\cdots +v_n)+d(v_1'+v_2'+\cdots +v_n')</mrow>
                    <mrow> \amp = cv_1+cv_2+\cdots +cv_n+dv_1'+dv_2'+\cdots +dv_n'</mrow>
                    <mrow> \amp =(cv_1+dv_1')+(cv_2+dv_2')+\cdots +(cv_n+dv_n')</mrow>
                    <mrow> \amp = v_1''+v_2''+\cdots v_n''</mrow>
                </md>,
                where <m>v_i''=cv_i+dv_i'</m> for all <m>1\leq i\leq n</m>. 
                Since each <m>W_i</m> is a subspace, we have 
                <me>v_i''=cv_i+dv_i'\in W_i</me>
                for all <m>1\leq i\leq n</m>. We conclude that <m>cw_1+dw_2\in W</m>, as desired. 
            </p>
        </li>
        <li>
            <p>
                For any <m>v\in W_i</m>, we have 
                <me>
                    v=v_1+v_2+\cdots +v_n
                </me>,
                where 
                <me>
                    v_j=\begin{cases}
                    \boldzero \amp \text{if } j\ne i \\
                    v \amp \text{if } j=i 
                    \end{cases}
                </me>.
                Since <m>v_j\in W_j</m> for all <m>1\leq j\leq n</m>, we see that <m>v\in W</m>. Since <m>v</m> was an arbitrary element of <m>W_i</m>, we conclude that <m>W_i\subseteq W</m> for all <m>1\leq i\leq n</m>.
            </p>
            <p>
                Now assume <m>U</m> is a subspace of <m>V</m> that contains <m>W_i</m> for all <m>1\leq i\leq n</m>. We will show that <m>W=\sum_{i=1}^n W_i\subseteq U</m>. Indeed, given any <m>v\in W</m>, we have 
                <me>
                    v=v_1+v_2+\cdots +v_n
                </me>
                for some vectors <m>v_1,v_2,\dots, v_n</m>, where <m>v_i\in W_i</m>. Since <m>W_i\subseteq U</m> for all <m>i</m>, we have <m>v_i\in U</m> for all <m>i</m>; since <m>U</m> is closed under addition, we have <m>v=v_1+v_2+\cdots +v_n\in U</m>, as desired. 
            </p>
        </li>
    </ol>
    </p>
    </proof>
    </theorem>
    <example xml:id="eg_sum_R3">
    <title>Sums of subspaces</title>
    <statement>
    <p>
    Let <m>V=\R^3</m> and consider the following subsets of <m>V</m>: 
    <md>
        <mrow>W_1 \amp = \{(r,0,0)\colon r\in \R\}</mrow>
        <mrow>W_2 \amp = \{(0,s,0)\colon s\in \R\}</mrow>
        <mrow>W_3 \amp = \{(t,t,0)\colon t\in \R\}</mrow>
    </md>.
    <ol>
        <li>
            <p>
                Prove that each <m>W_i</m> is a subspace of <m>\R^3</m>. 
            </p>
        </li>
        <li>
            <p>
                Identify <m>W_1+W_2</m> as a familiar subspace of <m>\R^3</m>. Justify your answer. 
            </p>
        </li>
        <li>
            <p>
                Identify <m>W_1+W_3</m> as a familiar subspace of <m>\R^3</m>. Justify your answer. 
            </p>
        </li>
        <li>
            <p>
                Identify <m>W_1+W_2+W_3</m> as a familiar subspace of <m>\R^3</m>. Justify your answer. 
            </p>
        </li>
    </ol>
    </p>
    </statement>
    <solution>
    <p>
   <ol>
    <li>
        <p>
            It is fairly clear that each <m>W_i</m> above contains the zero vector and is closed under addition and scalar multiplication. We leave a careful proof of these facts to the reader. 
        </p>
    </li>
    <li>
        <p>
            Let <m>W=\{(a,b,0)\colon a,b\in \R\}</m>, the <m>xy</m>-plane. Claim: <m>W_1+W_2=W</m>. We prove both inclusions of this set equality separately.  
        </p>
        <p>
            Given <m>v\in W_1+W_2</m>, we have <m>v=v_1+v_2</m> for some <m>v_1=(a,0,0)\in W_1</m> and <m>v_2=(0,b,0)\in W_2</m>. But then 
            <me>
                v=(a,0,0)+(0,b,0)=(a,b,0)\in W
            </me>.
            Thus <m>W_1+W_2\subseteq W</m>.
        </p>
        <p>
            For the other direction, given any <m>v=(a,b,0)\in W</m>, we have 
            <me>
                v=(a,0,0)+(0,b,0)\in W_1+W_2
            </me>.
            Thus <m>W\subseteq W_1+W_2</m>, and we conclude <m>W=W_1+W_2</m>.
        </p>
    </li>
    <li>
        <p>
            Claim: <m>W_1+W_3=W</m>, with <m>W</m> as above. The inclusion <m>W_1+W_3\subseteq W</m> is obvious and can be proved just as above. The reverse inclusion requires a little more work. 
        </p>
        <p>
            Given <m>v=(a,b,0)\in W</m> we must show that there are elements <m>v_1=(r,0,0)\in W_1</m> and <m>v_2=(s,s,0)\in W_3</m> satisfying
            <me>
                v=(a,b,0)=(r,0,0)+(s,s,0)=(r+s,s,0)
            </me>.
            Equating coordinates we see that we want to find a solution <m>(r,s)</m> to the linear system
            <md>
                <mrow>r+s \amp = a</mrow>
                <mrow>s \amp =b</mrow>
            </md>,
            where <m>a</m> and <m>b</m> are given. We easily solve to conclude that there is in fact exactly one solution: <m>r=a-b, s=b</m>. In particular we have 
            <me>
                v=(a,b,0)=(a-b,0,0)+(b,b,0)\in W_1+W_3
            </me>.
            This proves <m>W\subseteq W_1+W_3</m> and hence that <m>W=W_1+W_3</m>.
        </p>
    </li>
    <li>
        <p>
            Claim: <m>W_1+W_2+W_3=W</m>, with <m>W</m> as above. First observe that since <m>W</m> is a subspace and <m>W_i\subseteq W</m> for all <m>1\leq i\leq 3</m>, we then have 
            <me>
                W_1+W_2+W_3\subseteq W
            </me>
            by (2) of <xref ref="th_subspace_sum"/>. For the other inclusion, observe that <m>W_1+W_2</m> by the first part, and thus 
            <me>
                W=W_1+W_2\subseteq W_1+W_2+W_3
            </me>.
            We conclude that <m>W=W_1+W_2+W_3</m>.
        </p>
    </li>
   </ol>
    </p>
    </solution>
    </example>
    <definition xml:id="d_subspace_direct_sum">
    <title>Direct sum of subspaces</title>
    <statement>
    <p>
    Let <m>W_1,W_2,\dots, W_n</m> be subspaces of the <m>F</m>-vector space <m>V</m>. We say <m>W</m> is the <term>direct sum</term> of the subspaces <m>W_i</m>, denoted 
    <men xml:id="eq_subspace_dir_sum">W=W_1\oplus W_2+\cdots \oplus W_n</men>,
    or <m>W=\bigoplus_{i=1}^n W_i</m>,  if the following conditions hold.
    <ol>
        <li>
            <p>
                <m>W=V_1+V_2+\cdots +V_n</m>.
            </p>
        </li>
        <li>
            <p>
                For each <m>v\in W</m> there is a unique choice of vectors <m>v_i\in W_i</m> such that 
                <men xml:id="eq_element_dir_sum">
                    v=v_1+v_2+\cdots +v_n
                </men>.
                In other words if we have 
                <me>
                    v_1+v_2+\cdots +v_n=v_1'+v_2'+\cdots +v_n'
                </me>,
                where <m>v_i,v_i'\in W_i</m> for all <m>1\leq i\leq n</m>, then 
                <me>
                    v_i=v_i'
                </me>
                for all <m>1\leq i\leq n</m>.
            </p>
        </li>
    </ol>
    We call <xref ref="eq_subspace_dir_sum"/> a <term>direct sum decomposition</term> of <m>W</m>. 
    </p>
    </statement>
    </definition>
    <example xml:id="eg_direct_sum_Rn">
    <title>Direct sum</title>
    <statement>
    <p>
    Let <m>V=\R^3</m> and consider the following subspaces of <m>V</m>: 
    <md>
        <mrow>W_1 \amp = \{(r,0,0)\colon r\in \R\}</mrow>
        <mrow>W_2 \amp = \{(0,s,0)\colon s\in \R\}</mrow>
        <mrow>W_3 \amp = \{(t,t,0)\colon t\in \R\}</mrow>
        <mrow>W \amp = \{(a,b,0)\colon a,b\in \R\}</mrow>
    </md>.
    <ol>
        <li>
            <p>
                Show that <m>W=W_1\oplus W_2</m> and <m>W=W_1\oplus W_3</m>. 
            </p>
        </li>
        <li>
            <p>
                Show that <m>W\ne W_1\oplus W_2\oplus W_3</m>. 
            </p>
        </li>
    </ol>
    </p>
    </statement>
    <solution>
    <p>
    <ol>
        <li>
            <p>
                We know already that <m>W=W_1+W_2=W_1+W_3</m> from <xref ref="eg_sum_R3"/>. Furthermore, it is clear by inspection that the decomposition
                <me>
                    (a,b,0)=v_1+v_2, v_1\in W_1, v_2=W_2
                </me>
                if and only if <m>v_1=(a,0,0)</m> and <m>v_2=(0,b,0)</m>, showing that <m>W=W_1\oplus W_2</m>. Furthermore, in <xref ref="eg_sum_R3"/> we showed that 
                <me>
                    (a,b,0)=v_1+v_3, v_1\in W_1, v_3\in W_3
                </me>
                if and only if <m>v_1=(a-b,0,0), v_2=(b,b,0)</m>. Thus <m>W=W_1\oplus W_3</m>.
            </p>
        </li>
        <li>
            <p>
                We know that <m>W=W_1+W_2+W_3</m> from <xref ref="eg_sum_R3"/>. To see that <m>W</m> is not the direct sum of the <m>W_i</m> it suffices to show one example of a vector <m>(a,b,0)\in W</m> that can be decomposed into a sum of elements of <m>W_1,W_2,W_3</m> in two distinct ways. Here is such an example:
                <md>
                    <mrow>(1,1,0) \amp =(0,0,0)+(0,0,0)+(1,1,0)</mrow>
                    <mrow> \amp =(1,0,0)+(0,1,0)+(0,0,0)</mrow>
                </md>.
            </p>
        </li>
    </ol>
    </p>
    </solution>
    </example>
    <example xml:id="eg_direct_sum_Fn">
    <title>Direct sum decomposition of <m>F^n</m></title>
    <statement>
    <p>
    Consider the space <m>F^n</m> of <m>n</m>-tuples with coefficients in <m>F</m>. For each <m>1\leq i\leq n</m>, let <m>W_i</m> be the set of all <m>n</m>-tuples of the form 
    <me>
        v=(0,\dots,0,\underset{i\text{-th coor.}}{a}, 0,\dots, 0), a\in F
    </me>.
    In other words <m>W_i</m> is the set of all <m>n</m>-tuples whose <m>j</m>-th coordinates are equal to zero for all <m>j\ne i</m>. 
    </p>
    <p>
        Prove that 
        <me>
            F^n=W_1\oplus W_2\cdots \oplus W_n
        </me>.
        You may take for granted that <m>W_i</m> is a subspace of <m>F^n</m> for all <m>i</m>. 
    </p>
    </statement>
    <solution>
    <p>
    Given <m>v=(a_1,a_2,\dots, a_n)\in F^n</m> we have 
    <men xml:id="eq_Fn_dir_sum">
        v=v_1+v_2+\cdots +v_n
    </men>,
    where 
    <me>
        v_i=(0,\dots, a_i,0,\dots, 0)\in W_i
    </me>.
    It follows that <m>F^n=\sum_{i=1}^n W_i</m>. Furthermore, the decomposition <xref ref="eq_Fn_dir_sum"/> is unique: if 
    <me>
        (a_1,a_2,\dots, a_n)=v_1'+v_2'+\cdots +v_n'
    </me>
    with <m>v_i'\in W_i</m> for all <m>i</m>, then since <m>v_i'</m> is the only vector with a nonzero <m>i</m>-th coordinate, we must have <m>v_i'=(0,\dots, 0,a_i,0,\dots,0)</m>. Since the decompotision <xref ref="eq_Fn_dir_sum"/> is unique, we conclude that <m>F^n=\bigoplus_{i=1}^nW_i</m>. 
    </p>
    </solution>
    </example>
    
    
    <theorem xml:id="th_subspace_direct_sum">
    <title>Direct sum of subspaces</title>
    <statement>
    <p>
    Let <m>W_1,W_2,\dots, W_n</m> be subspaces of the <m>F</m>-vector space <m>V</m>, and let <m>W=\sum_{i=1}^n W_i</m>. The following statements are equivalent. 
    <ol>
        <li>
            <p>
                <m>W=\bigoplus_{i=1}^n W_i</m>
            </p>
        </li>
        <li>
            <p>
                If <m>\boldzero=v_1+v_2+\cdots +v_n</m> with <m>v_i\in W_i</m> for all <m>1\leq i\leq n</m>, then <m>v_i=\boldzero</m> for all <m>1\leq i\leq n</m>. Using logical shorthand: 
                <men xml:id="eq_dir_sum_equiv">
                 \boldzero=v_1+v_2+\cdots +v_n, v_i\in W_i\implies v_1=v_2\cdots =v_n=\boldzero   
                </men>.
            </p>
        </li>
    </ol>
    </p>
    </statement>
    <proof>
    <p>
        Since the premises include the assumption that <m>W=\sum_{i=1}^n W_i</m> we need only show that condition (ii) of <xref ref="d_subspace_direct_sum"/> is equivalent to condition <xref ref="eq_dir_sum_equiv"/>. We prove both implications separately.  
    </p>
    <p>
        Suppose condition (ii) of <xref ref="d_subspace_direct_sum"/> is satisfied. Since <m>\boldzero=\boldzero+\boldzero+\cdots +\boldzero</m> is one decomposition of <m>\boldzero</m> into elements of the <m>W_i</m>, and since (ii) asserts such decompositions are unique, we conclude that <xref ref="eq_dir_sum_equiv"/> holds. 
    </p>
    <p>
        Assume <xref ref="eq_dir_sum_equiv"/> holds, and suppose we have 
        <me>
            v=v_1+v_2+\cdots +v_n=v_1'+v_2'+\cdots +v_n'
        </me>
        with <m>v_i, v_i'\in W_i</m>. It follows, after a little algebra, that 
        <me>
            (v_1-v_1')+(v_2-v_2')+\cdots +(v_n-v_n')=\boldzero
        </me>.
        Since we assume condition <xref ref="eq_dir_sum_equiv"/>, we conclude that <m>v_i-v_i'=\boldzero</m> for all <m>1\leq i\leq n</m>, or equivalently, <m>v_i=v_i'</m> for all <m>1\leq i\leq n</m>, as desired.
    </p>
    </proof>
    </theorem>
    <corollary xml:id="cor_subspace_dir_sum">
        <statement>
            <p>
                Let <m>W_1</m> and <m>W_2</m> be subspaces of the <m>F</m>-vector space <m>V</m>, and let <m>W=W_1+W_2</m>. The following statements are equivalent. 
                <ol>
                    <li>
                        <p>
                            <m>W=W_1\oplus W_2</m>.
                        </p>
                    </li>
                    <li>
                        <p>
                            <m>W_1\cap W_2=\{\boldzero\}</m>.
                        </p>
                    </li>
                </ol>
            </p>
        </statement>
        <proof>
            <p>
                We prove both implications separately. 
            </p>
            <case>
            <title>Implication: (1)<m>\implies</m>(2)</title>
            <p>
            Assume <m>W=W_1\oplus W_2</m>. Since <m>0\in W_i</m> for <m>1\leq i\leq 2</m>, we have <m>\{\boldzero\}\subseteq W_1\cap W_2</m>. It remains to prove the reverse inclusion <m>W_1\cap W_2\subseteq \{\boldzero\}</m>. Given <m>v\in W_1\cap W_2</m>, we have <m>v\in W_1</m> and <m>-v\in W_2</m>, and thus 
            <me>
                \boldzero=v+ (-v)
            </me>
            is a decomposition of <m>\boldzero</m> in terms of <m>W_1</m> and <m>W_2</m>. Since <m>W=W_1\oplus W_2</m>, we conclude from <xref ref="th_subspace_direct_sum"/> that <m>v=-v=\boldzero</m>. Thus <m>W_1\cap W_2=\{\boldzero\}</m>.
            </p>
            </case>
            <case>
            <title>Implication: (2)<m>\implies</m>(1)</title>
            <p>
            Now assume <m>W_1\cap W_2=\{\boldzero\}</m>. Using <xref ref="th_subspace_direct_sum"/>, it suffices to show that if <m>\boldzero=v_1+v_2</m> with <m>v_1\in W_1</m> and <m>v_2\in W_2</m>, then <m>v_1=v_2=\boldzero</m>. If <m>\boldzero=v_1+v_2</m> with <m>v_i\in W_i</m>, then we have 
            <md>
                <mrow> v_1\amp =-v_2\in W_2 </mrow>
                <mrow>v_2 \amp =-v_1\in W_1</mrow>
            </md>, 
            and hence that <m>v_1\in W_1\cap W_2</m> and <m>v_2\in W_1\cap W_2</m>. 
            Since <m>W_1\cap W_2=\{\boldzero\}</m>, we conclude that <m>v_1=v_2=\boldzero</m>, as desired. 
            
            </p>
            </case>
            
            
        </proof>
    </corollary>
    <definition xml:id="d_matrix_notation">
<title>Matrix notation</title>
  <notation>
    <usage><m>[a_{ij}]_{m\times n}</m></usage>
    <description>Matrix whose <m>ij</m>-th entry is <m>a_{ij}</m></description>
  </notation>
  <notation>
    <usage><m>(A)_{ij}</m></usage>
    <description><m>ij</m>-th entry of the matrix <m>A</m></description>
  </notation>
  <statement>
    <p>
        Let <m>F</m> be a field.  We adopt the following notation for matrices of <m>F^{m,n}</m>. 
      <ul>
      <li>
        <title>Matrix-building notation</title>
        
        <p>
          The notation <m>[a_{ij}]_{m\times n}</m> denotes the
           matrix of <m>F^{m,n}</m> whose <m>ij</m>-th entry is <m>a_{ij}</m> for all <m>1\leq i\leq m</m> and <m>1\leq j\leq n</m>. When there is no danger of confusion, this notation will be shortened to <m>[a_{ij}]</m>.
        </p>
      </li>
      <li>
        <title>Matrix entry notation</title>
        <p>
          Given a matrix <m>A\in F^{m,n}</m>, for all <m>1\leq i\leq m</m> and <m>1\leq j\leq n</m>, 
          <m>[A]_{ij}</m> denotes the <m>ij</m>-th entry of <m>A</m>.
        </p>
      </li>
    </ul>
    </p>
  </statement>
</definition>
    <definition xml:id="d_transpose">
    <title>Transpose matrix</title>
    <statement>
    <p>
    Given a matrix <m>A\in F^{m,n}</m>, its <term>transpose</term> is the matrix <m>A^T\in F^{n,m}</m> whose <m>ij</m>-th entry is the <m>ji</m>-th entry of <m>A</m> for all <m>1\leq i\leq n, 1\leq j\leq m</m>. In other words, <m>A^T</m> is the unique matrix of <m>F^{n,m}</m> satisfying 
    <me>
        [A^T]_{ij}=[A]_{ji}
    </me>
    for all <m>1\leq i\leq n</m> and <m>1\leq j\leq m</m>. 
    </p>
    </statement>
    </definition>
    
    <example xml:id="eg_direct_sum_matrices">
    <title>Direct sum of matrix spaces</title>
    <statement>
    <p>
    Let <m>V=F^{2,2}</m>, the space of all <m>2\times 2</m> matrices with entries in <m>F</m>, and consider the following subsets of <m>V</m>: 
    <md>
        <mrow>W_1 \amp =\{A\in F^{2,2}\colon A^T=A\}</mrow>
        <mrow>W_2 \amp = \{A\in F^{2,2}\colon A^T=-A\}</mrow>
    </md>.
    In other words, <m>W_1</m> is the set of all symmetric matrices of <m>F^{2,2}</m> and <m>W_2</m> is the set of all skew-symmetric matrices of <m>F^{2,2}</m>. 
    <ol>
        <li>
            <p>
                Prove that <m>W_1</m> and <m>W_2</m> are subspaces of <m>F^{2,2}</m>. 
            </p>
        </li>
        <li>
            <p>
                Prove that <m>F^{2,2}=W_1\oplus W_2</m>. 
            </p>
        </li>
    </ol>
    </p>
    </statement>
    <solution>
    <p>
    <ol>
        <li>
            <p>
                Using the defining conditions <m>A^T=A</m> and <m>A^T=-A</m>, it is easy to see that 
                <md>
                    <mrow>W_1 \amp =\left\{\begin{bmatrix}
                    a\amp b \\ b\amp c\end{bmatrix}\colon a,b,c\in F\right\}
                    </mrow>
                    <mrow>W_2 \amp =\left\{\begin{bmatrix}
                    0\amp b \\ -b\amp 0\end{bmatrix}\colon b\in F\right\}
                    </mrow>
                </md>.
                From these descriptions it follows easily that <m>W_1</m> and <m>W_2</m> contain the zero matrix, and are closed under addition and scalar multiplication. We leave the details to the reader. 
            </p>
        </li>
        <li>
            <p>
                Let <m>W=W_1+W_2</m>. First we show that <m>W=W_1\oplus W_2</m>. To do so, it suffices to show <m>W_1\cap W_2=\{\boldzero\}</m> by <xref ref="cor_subspace_dir_sum"/>. But this is clear from the parametric descriptions of <m>W_1</m> and <m>W_2</m> given above. 
            </p>
            <p>
                Next we show that <m>W=F^{2,2}</m>. By definition we have <m>W=W_1+W_2\subseteq F^{2,2}</m>, so we need only show the reverse inclusion. Given an arbitrary matrix <m>A\in F^{2,2}</m>, we must show that we can write <m>A=A_1+A_2</m> where <m>A_1\in W_1</m> and <m>A_2\in W_2</m>. In other words, we must show that any matrix can be written as a sum of a symmetric matrix and a skew-symmetric matrix. This can be done essentially by inspection in this low-dimensional case (<m>n=2</m>):  we have 
                <me>
                   \begin{bmatrix}
                a\amp b\\ c\amp d
                \end{bmatrix} =\frac{1}{2}\begin{bmatrix}
                2a\amp b+c \\ b+c \amp 2d
                \end{bmatrix}+
                \frac{1}{2}\begin{bmatrix}
                0\amp b-c \\ -b+c \amp 0
                \end{bmatrix}
                </me>
                for any matrix <m>A=\begin{bmatrix}
                a\amp b\\ c\amp d
                \end{bmatrix}</m>. This fact is true more generally, however, and so it is worth adding an argument that works for all <m>n</m>: namely, observe that <m>A=A_1+A_2</m>, where 
                <md>
                    <mrow>A_1 \amp =\frac{1}{2}(A+A^T)</mrow>
                    <mrow>A_2 \amp =\frac{1}{2}(A-A^T)</mrow>
                </md>.
                Using elementary properties of transpose, it is now easy to show that <m>A_1^T=A_1</m> and <m>A_2^T=-A_2</m>: <ie/>, <m>A_1\in W_1</m> and <m>A_2\in W_2</m>. We will remind you of these elementary properties of the transpose operator later on. 
            </p>
        </li>
    </ol>
    </p>
    </solution>
    </example>
    

</section>