<?xml version="1.0" encoding="UTF-8"?>

<section xml:id="s_vector_space_functions" xmlns:xi="http://www.w3.org/2001/XInclude">
    <title>Vector spaces (cont.)</title>
<subsection xml:id="">
<title>Function spaces</title>
<p>
    As promised, we now prove that sets <m>F^n</m>, <m>F^\infty</m>, <m>F^{m,n}</m>, together with their indicated operations, do indeed satisfy the vector space axioms. We will do this in a somewhat indirect manner by first constructing a more general vector space <m>F^I</m>, and then showing that <m>F^n</m>, <m>F^\infty</m>, and <m>F^{m,n}</m> are just specific instances of this more general construction, corresponding to particular choices of the set <m>I</m>. 
</p>
<p>
    The objects of the vector space <m>F^I</m> defined in <xref ref="d_tuple_space"/> can be thought of either as functions <m>f\colon I\rightarrow F</m> from the set <m>I</m> to the field <m>F</m>, or equivalently, as <m>F</m>-valued tuples <m>(a_i)_{i\in I}</m> indexed by <m>I</m>. Hence the <q>functions/tuples</q> in its name. Depending on the context, one of these two equivalent conceptions (function or tuple) may be more convenient than the other. For example, to make the connection between <m>F^I</m>, <m>F^n</m>, <m>F^\infty</m>, and <m>F^{m,n}</m>, it is most convenient to think in terms of tuples. See <xref ref="d_Ituple"/> for the general definition of tuples and <xref ref="rm_tuple_function"/> for an explication of the equivalence between functions and tuples.   
</p>
<definition xml:id="d_tuple_space">
<title>Space of <m>F</m>-valued functions/tuples</title>
<statement>
<p>
Let <m>F</m> be a field. Given any set <m>I</m>, recall that <m>F^I</m> is defined as the set of all functions <m>f\colon I\rightarrow F</m>: <ie/> 
<me>F^I=\{f\colon I\rightarrow F\}</me>. 
Equivalently, thinking of functions as tuples, we can describe <m>F^I</m> as the set of all <m>F</m>-valued tuples indexed by <m>I</m>: <ie/>, 
<me>
    F^I=\{(a_i)_{i\in I}\colon a_i\in F\}
</me>.
Below we define a vector space structure on <m>F^I</m>. 
<ul>
    <li>
        <title>Vector operations</title>
        <p>
            Given elements <m>f=(f(i))_{i\in I}, g=(g(i))_{i\in I}\in F^I</m> and scalar <m>c\in F</m>, we define 
            <md>
                <mrow>f+g \amp = (f(i)+g(i))_{i\in I}</mrow>
                <mrow>cf \amp =(cf(i))_{i\in I}</mrow>
            </md>.
            In other words, <m>f+g</m> is the function defined as <m>(f+g)(i)=f(i)+g(i)</m> for all <m>i\in I</m>, and <m>cf</m> is the function defined as <m>(cf)(i)=cf(i)</m> for all <m>i\in I</m>. 
        </p>
    </li>
    <li>
        <title>Zero vector</title>
        <p>
            The zero vector of <m>F^I</m> is the zero function <m>0_I\colon I\rightarrow F</m> defined as <m>0_I(i)=0</m> for all <m>i\in I</m>. In other words, using tuple notation, we have <m>\boldzero=0_I=(0)_{i\in I}</m>. 
        </p>
    </li>
    <li>
        <title>Vector inverses</title>
        <p>
            Given an element <m>f=(f(i))_{i\in I}\in F^I</m> its vector inverse <m>-f</m> is defined as 
            <me>
                -f=(-f(i))_{i\in I}
            </me>.
            In other words <m>-f</m> is the function on <m>I</m> defined as <m>(-f)(i)=-f(i)</m> for all <m>i\in I</m>.
        </p>
    </li>
</ul>
We call <m>F^I</m>, together with these vector operations, the <term>space of functions from <m>I</m> to <m>F</m></term>, or, thinking in terms of tuples, the <term>space of <m>F</m>-valued tuples indexed by <m>I</m></term>.
</p>
</statement>
</definition>
<theorem xml:id="th_vs_egs">
<title>Function/tuple spaces are vector spaces</title>
<statement>
<p>
Each of the sets <m>F^n</m>, <m>F^\infty</m>, <m>F^{m,n}</m>, <m>F^I</m>, together with the accompanying vector operations defined above, is a vector space. 
</p>
</statement>
<proof>
    <p>
        First we observe, thinking in terms of tuples, that each of the sets <m>F^{n}</m>, <m>F^\infty</m>, <m>F^{m,n}</m>, along with their accompanying vector space operations, is a specific example of <m>F^I</m> together with its vector operations. This is seen by choosing an appropriate index set <m>I</m> in each case. In more detail, we have 
        <md>
            <mrow> F^n\amp= F^I, \text{ where } I=\{1,2,\dots, n\} </mrow>
            <mrow> F^\infty\amp= F^I, \text{ where } I=\Z_+=\{1,2,3,\dots\} </mrow>
            <mrow> F^{m,n}\amp= F^I, \text{ where } I=\{(i,j)\colon 1\leq i\leq m, 1\leq j\leq n\} </mrow>
        </md>.
        Thus it suffices to show that <m>F^I</m> is a vector space with respect to the given vector operations. 
        To do this, we follow <xref ref="proc_vector_space"/>. Since <xref ref="d_tuple_space"/> has already taken care of steps (1)-(3) for us, it remains to show that the vector space axioms are satisfied. As you will see, the tuple notation for functions makes these proofs quite straightforward consequences of the field axioms satisfied by <m>F</m>.
        </p>
        <p> 
            Consider the arithmetic axioms first. We will verify that Axioms (i), (ii), and (v) are satisfied. Given <m>f=(f(i))_{i\in I},g=(g(i))_{i\in I},h=(h(i))_{i\in I}\in F^I</m> and <m>c\in F</m>, we have 
        <md>
            <mrow> f+g \amp = (f(i)+g(i))_{i\in I} \amp (\text{def. vec. add.}) </mrow>
            <mrow> \amp = (g(i)+f(i))_{i\in I} \amp (\text{field prop.})</mrow>
            <mrow> \amp = g+f \amp (\text{def. vec. add.})</mrow>
            <mrow> \amp </mrow>
            <mrow>f+(g+h) \amp = (f(i)+(g+h)(i))_{i\in I} \amp (\text{def. vec. add.})</mrow>
            <mrow> \amp = (f(i)+(g(i)+h(i)))_{i\in I} \amp (\text{def. vec. add.})</mrow>
            <mrow> \amp = ((f(i)+g(i))+h(i))_{i\in I} \amp (\text{field prop.})</mrow>
            <mrow> \amp = ((f+g)(i)+h(i))_{i\in I} \amp  (\text{def. vec. add.})</mrow>
            <mrow> \amp = (f+g)+h \amp  (\text{def. vec. add.})</mrow>
            <mrow> \amp </mrow>
            <mrow>c(f+g) \amp =(c(f+g)(i))_{i\in I} \amp (\text{def. scal. mult})</mrow>
            <mrow> \amp = (c(f(i)+g(i)))_{i\in I} \amp (\text{def. vec. add.})</mrow>
            <mrow> \amp = (cf(i)+cg(i))_{i\in I} \amp (\text{field prop.})</mrow>
            <mrow> \amp =((cf)(i)+(cg)(i))_{i\in I} \amp (\text{def. scal. mult})</mrow>
            <mrow> \amp = cf+cg \amp (\text{def. vec. add.})</mrow>
        </md>.
        Lastly we will show that <m>0_I</m> does indeed satisfy the additive identity axiom (Axiom (iii)), leaving the verification of Axiom (iv) to the reader. Given any element <m>f=(f(i))_{i\in I}\in F^I</m>, we have 
        <md>
            <mrow>0_I+f \amp =(0_I(i)+f(i))_{i\in I} \amp (\text{def. vec. add.})</mrow>
            <mrow> \amp = (0+f(i))_{i\in I}\amp (\text{def. of } 0_I)</mrow>
            <mrow> \amp = (f(i))_{i\in I} \amp (\text{field prop.})</mrow>
            <mrow> \amp = f</mrow>
        </md>,
        as desired. 
    </p>
</proof>
</theorem>


<example xml:id="eg_real_functions">
<title>Real-valued functions</title>
<statement>
<p>
Let <m>I=[a,b]\subseteq \R </m> be an interval in the real line. Using the function interpretation of <m>F^I</m>, <m>\R^{[a,b]}</m> is the set of all functions of the form <m>f\colon [a,b]\rightarrow \R</m>. The vector operations defined in <xref ref="d_tuple_space"/> in this setting correspond to the function-arithmetic operations you met in precalculus and calculus: <ie/>, given functions <m>f,g\in \R^{[a,b]}</m>, their vector sum <m>f+g</m> is the function defined as 
<m>(f+g)(x)=f(x)+g(x)</m> for all <m>x\in [a,b]</m>. Similarly, given a scalar <m>c\in \R</m> and function <m>f\in \R^{[a,b]}</m>, the vector scalar multiple <m>cf</m> is the function defined as <m>(cf)(x)=cf(x)</m> for all <m>x\in \R</m>. 
</p>
<p>
    In this context it is possible to visualize our vector operations in terms of the graphs of the functions on the interval <m>[a,b]</m>. 
</p>
<figure xml:id="fig_func_arith">
    <caption>Visualizing function arithmetic in <m>\R^{[-1,1]}</m></caption>
    <sidebyside>
        <figure xml:id="fig_func_add">
        <caption>Visualizing <m>f+g</m></caption>
        <image>
            <shortdescription>Visualizing function addition</shortdescription>
           <sageplot>
        f=plot(x,x,-1,1,color="blue")
        g=plot(sin(pi*x),x,-1,1,color="red")
        h=plot(x+sin(pi*x),x,-1,1,color="green")
        s=text("$f$",(.5,.7),color="black",fontsize=16)
        r=text("$g$",(.5,1.2),color="black",fontsize=16)
        t=text("$f+g$",(.5,1.7),color="black",fontsize=16)
        f+g+h+s+r+t
        </sageplot> 
        </image>
        </figure>
         <figure xml:id="fig_func_scale">
        <caption>Visualizing <m>cf</m></caption>
        <image>
            <shortdescription>Visualizing function scalar multiplication</shortdescription>
           <sageplot>
        f=plot(sin(pi*x),x,-1,1,color="blue")
        g=plot(.5*sin(pi*x),x,-1,1,color="red")
        h=plot(-1.5*sin(pi*x),x,-1,1,color="green")
        s=text("$\\frac{1}{2}\\,f$",(.5,.7),color="black",fontsize=16)
        r=text("$f$",(.5,1.2),color="black",fontsize=16)
        t=text("$-\\frac{3}{2}\\, f$",(.5,-1.3),color="black",fontsize=16)
        f+g+h+s+r+t
        </sageplot> 
        </image>
        </figure>
    </sidebyside>
</figure>

</statement>
</example>

</subsection>
<subsection xml:id="">
<title>Vector space properties</title>
<p>
    We end this section with a few elementary vector space properties. Since these statements involve a general vector space (as opposed to a specific type of vector space), we will make no assumptions about <m>V</m> and the base field <m>F</m>, other than that <m>V</m> satisfies the vector space axioms and <m>F</m> satisfies the field axioms. 
</p>
<theorem xml:id="th_zero_inv_unique">
<title>Uniqueness of zero vector and inverses</title>
<statement>
<p>
Let <m>V</m> be an <m>F</m>-vector space. 
<ol>
    <li>
        <p>
            The zero vector in <m>V</m> is unique: <ie/>, there is one and only one element of <m>V</m> that satisfies <xref ref="eq_zero_vector"/>.
        </p>
    </li>
    <li>
        <p>
            Inverse vectors are unique: <ie/>, for all <m>v\in V</m> there is one and only one vector <m>-v</m> satisfying <xref ref="eq_vec_inv"/>.
        </p>
    </li>
</ol>
</p>
</statement>
<proof>
<p>
    <ol>
        <li>
            <p>
                If <m>w\in V</m> satisfies <m>w+v=v</m> for all <m>v\in V</m>, then in particular, taking <m>v=\boldzero</m>, we see that <m>w+\boldzero=\boldzero</m>. But since <m>w+\boldzero=w</m> (using the defining property of <m>\boldzero)</m>, we see that 
                <md>
                    <mrow>w+\boldzero=\boldzero \amp \implies w=\boldzero</mrow>
                </md>.
                We conclude that <m>w=\boldzero</m>, as desired. 
            </p>
        </li>
        <li>
            <p>
                Let <m>v\in V</m>. Given <m>w\in V</m> we have 
                <md>
                    <mrow>w+v =\boldzero \amp \implies w+v=-v+v \amp (-v+v=\boldzero) </mrow>
                    <mrow> \amp \implies w+v+(-v)=-v+v+(-v)</mrow>
                    <mrow> \amp \implies w+\boldzero=-v+\boldzero \amp (v+(-v)=\boldzero)</mrow>
                    <mrow> \amp \implies w=-v \amp (\text{prop. of } \boldzero)</mrow>
                </md>. 
            </p>
        </li>
    </ol>

</p>
</proof>
</theorem>



<theorem xml:id="th_vs_props">
<title>Vector space properties</title>
<statement>
<p>
Let <m>V</m> be an <m>F</m>-vector space. 
 <ol>
    <li>
        <p>
            For all <m>v\in V</m>, we have <m>0\boldv=\boldzero</m>.
        </p>
    </li>

    <li>
        <p>
            For all <m>c\in F</m>, we have <m>c\boldzero=\boldzero</m>.
        </p>
    </li>

    <li>
        <p>
            For all <m>v\in V</m>, we have <m>(-1)\boldv=-\boldv</m>.
        </p>
    </li>

    <li>
        <p>
            For all <m>v\in V</m> and <m>c\in F</m>, if <m>cv=\boldzero</m>, then <m>c=0</m> or <m>v=\boldzero</m>.
        </p>
    </li>
</ol>
</p>
</statement>
<proof>
<p>
    We provide proofs of (1) and (3), leaving (2) and (4) to the reader. 
</p>
<p>
  Our proof of (1) is almost identical to a similar statement in <xref ref="th_field_props"/>. For any <m>v\in V</m>, we have 
  <md>
    <mrow>0v \amp = (0+0)v \amp (\text{field prop. of } F)</mrow>
    <mrow> \amp 0v+0v \amp (\text{dist. prop. of } V)</mrow>
  </md>.
  But then we have 
  <md>
        <mrow>0v\amp = 0v+0v </mrow>
        <mrow>-(0v)+0v\amp=-(0v)+0v+0v \amp (\text{add } -(0v)\text{ to both sides}) </mrow>
        <mrow>  \boldzero\amp=\boldzero+0v \amp (\text{vec. inv. prop.})</mrow>
        <mrow> \boldzero\amp=0v \amp (\text{prop. of } \boldzero)</mrow>
    </md>,
    as desired.
</p>
<p>
    Let <m>v\in V</m>. To prove (2), we will show that <m>(-1)v</m> satisfies the defining property <xref ref="eq_vec_inv"/> of <m>-v</m>; since each vector has a unique vector inverse (<xref ref="th_zero_inv_unique"/>), it will then follow that <m>(-1)v=-v</m>. To show <m>(-1)v</m> satisfies <xref ref="eq_vec_inv"/>, we observe that 
    <md>
        <mrow>(-1)v+v \amp =(-1)v+1v \amp (\text{Axiom (viii)})</mrow>
        <mrow> \amp = (-1+1)v \amp (\text{Axiom (vii)})</mrow>
        <mrow> \amp =0v</mrow>
        <mrow> \amp = \boldzero (\text{by (1)})</mrow>
    </md>.
    Thus <m>(-1)v=-v</m>. 
</p>
</proof>
</theorem>

</subsection>
    

</section>